code/experimental/ed25519/Hacl.Impl.Ed25519.Ladder.fst
@@ -9,12 +9,19 @@ open Lib.Buffer
 
 open Hacl.Bignum25519
 
+module S = Hacl.Spec.Ed25519.Field56.Definition
+module F = Hacl.Impl.Ed25519.Field56
+
+#set-options "--z3rlimit 20 --max_fuel 0 --max_ifuel 0"
+
 inline_for_extraction noextract
 val make_point_inf:
   b:lbuffer uint64 20ul ->
   Stack unit
     (requires fun h -> live h b)
-    (ensures  fun h0 _ h1 -> modifies (loc b) h0 h1)
+    (ensures  fun h0 _ h1 -> modifies (loc b) h0 h1 /\
+      F.point_eval h1 b == Spec.Curve25519.(zero, one, one, zero)
+    )
 let make_point_inf b =
   let x = sub b 0ul 5ul in
   let y = sub b 5ul 5ul in
@@ -30,7 +37,10 @@ val make_g:
   g:point ->
   Stack unit
     (requires fun h -> live h g)
-    (ensures fun h0 _ h1 -> modifies (loc g) h0 h1)
+    (ensures fun h0 _ h1 -> modifies (loc g) h0 h1 /\
+      F.point_eval h1 g == Spec.Ed25519.g
+    )
+
 let make_g g =
   let gx = getx g in
   let gy = gety g in
@@ -39,7 +49,8 @@ let make_g g =
   make_u64_5 gx (u64 0x00062d608f25d51a) (u64 0x000412a4b4f6592a) (u64 0x00075b7171a4b31d) (u64 0x0001ff60527118fe) (u64 0x000216936d3cd6e5);
   make_u64_5 gy (u64 0x0006666666666658) (u64 0x0004cccccccccccc) (u64 0x0001999999999999) (u64 0x0003333333333333) (u64 0x0006666666666666);
   make_one gz;
-  make_u64_5 gt (u64 0x00068ab3a5b7dda3) (u64 0x00000eea2a5eadbb) (u64 0x0002af8df483c27e) (u64 0x000332b375274732) (u64 0x00067875f0fd78b7)
+  make_u64_5 gt (u64 0x00068ab3a5b7dda3) (u64 0x00000eea2a5eadbb) (u64 0x0002af8df483c27e) (u64 0x000332b375274732) (u64 0x00067875f0fd78b7);
+  admit()
 
 inline_for_extraction noextract
 val ith_bit:
@@ -47,7 +58,9 @@ val ith_bit:
   -> i:size_t{v i < 256} ->
   Stack uint8
     (requires fun h -> live h k)
-    (ensures fun h0 z h1 -> h0 == h1 /\ v z <= 1)
+    (ensures fun h0 z h1 -> h0 == h1 /\ v z <= 1 /\
+        z == Spec.Ed25519.ith_bit (as_seq h0 k) (v i)
+    )
 let ith_bit k i =
   let q = i >>. 3ul in
   let r = i &. 7ul in
@@ -60,7 +73,6 @@ let ith_bit k i =
   uintv_extensionality (u8 1) (mod_mask #U8 1ul);
   z
 
-
 inline_for_extraction noextract
 val loop_step:
     b:lbuffer uint64 80ul
@@ -68,13 +80,25 @@ val loop_step:
   -> ctr:size_t{v ctr < 256} ->
   Stack unit
     (requires fun h -> live h b /\ live h k /\ disjoint k b)
-    (ensures  fun h0 _ h1 -> modifies (loc b) h0 h1)
+    (ensures  fun h0 _ h1 -> modifies (loc b) h0 h1 /\
+      (F.point_eval h1 (gsub b 0ul 20ul), F.point_eval h1 (gsub b 20ul 20ul)) ==
+      Spec.Ed25519.ladder_step (as_seq h0 k) (v ctr)
+       (F.point_eval h0 (gsub b 0ul 20ul), F.point_eval h0 (gsub b 20ul 20ul))
+    )
+
+#set-options "--z3rlimit 60"
+
+let lemma_to_u8_to_u64 (i:uint8) : Lemma (to_u8 (to_u64 i) == i)
+  = ()
+
 let loop_step b k ctr =
   let nq    = sub b 0ul 20ul in
   let nqpq  = sub b 20ul 20ul in
   let nq2   = sub b 40ul 20ul in
   let nqpq2 = sub b 60ul 20ul in
-  let i  = ith_bit k ctr in
+  let i  = ith_bit k (255ul -. ctr) in
+  (**) assert (v (255ul -. ctr) == 255 - v ctr);
+  (**) lemma_to_u8_to_u64 i;
   Hacl.Impl.Ed25519.SwapConditional.swap_conditional_inplace nq nqpq (to_u64 i);
   Hacl.Impl.Ed25519.PointDouble.point_double nq2 nq;
   Hacl.Impl.Ed25519.PointAdd.point_add nqpq2 nq nqpq;
@@ -85,13 +109,37 @@ val point_mul_:
     b:lbuffer uint64 80ul
   -> k:lbuffer uint8 32ul ->
   Stack unit
-    (requires fun h -> live h k /\ live h b /\ disjoint b k)
-    (ensures  fun h0 _ h1 -> modifies (loc b) h0 h1)
+    (requires fun h -> live h k /\ live h b /\ disjoint b k /\
+      F.point_eval h (gsub b 0ul 20ul) == Spec.Curve25519.(zero, one, one, zero)
+    )
+    (ensures  fun h0 _ h1 -> modifies (loc b) h0 h1 /\
+       F.point_eval h1 (gsub b 0ul 20ul) ==
+       Spec.Ed25519.point_mul (as_seq h0 k) (F.point_eval h0 (gsub b 20ul 20ul))
+    )
+
+#set-options "--z3rlimit 60 --max_fuel 0 --max_ifuel 0"
+
 let point_mul_ b k =
   let h0 = ST.get() in
-  let inv h (i:nat{i <= 256}) = modifies (loc b) h0 h in
+
+  [@inline_let]
+  let spec h0 = Spec.Ed25519.ladder_step (as_seq h0 k) in
+
+  [@inline_let]
+  let acc h : GTot (Spec.Ed25519.ext_point & Spec.Ed25519.ext_point) =
+    F.point_eval h (gsub b 0ul 20ul), F.point_eval h (gsub b 20ul 20ul)
+  in
+
+  [@inline_let]
+  let inv h (i:nat{i <= 256}) = modifies (loc b) h0 h /\
+    acc h == Lib.LoopCombinators.repeati i (spec h0) (acc h0)
+  in
+
+  Lib.LoopCombinators.eq_repeati0 256 (spec h0) (acc h0);
   Lib.Loops.for 0ul 256ul inv
-    (fun i -> loop_step b k (256ul -. i -. 1ul))
+    (fun i ->
+      Lib.LoopCombinators.unfold_repeati 256 (spec h0) (acc h0) (v i);
+      loop_step b k i)
 
 val point_mul:
     result:point
@@ -99,7 +147,10 @@ val point_mul:
   -> q:point ->
   Stack unit
     (requires fun h -> live h scalar /\ live h q /\ live h result)
-    (ensures  fun h0 _ h1 -> modifies (loc result) h0 h1)
+    (ensures  fun h0 _ h1 -> modifies (loc result) h0 h1 /\
+      F.point_eval h1 result == Spec.Ed25519.point_mul (as_seq h0 scalar) (F.point_eval h0 q)
+    )
+
 let point_mul result scalar q =
   push_frame();
   let b = create 80ul (u64 0) in
@@ -117,7 +168,9 @@ val point_mul_g:
   Stack unit
     (requires fun h ->
       live h scalar /\ live h result /\ disjoint result scalar)
-    (ensures  fun h0 _ h1 -> modifies (loc result) h0 h1)
+    (ensures  fun h0 _ h1 -> modifies (loc result) h0 h1 /\
+      F.point_eval h1 result == Spec.Ed25519.point_mul (as_seq h0 scalar) Spec.Ed25519.g
+    )
 let point_mul_g result scalar =
   push_frame();
   let g = create 20ul (u64 0) in
